Bytes.v
@@ -1,9 +1,10 @@
-Require Import DecidableEquality.
 (** Bytes is an axiomatic library for byte strings. *)
+
+Require Import EquivDec.
 
 (* bytes n is a byte string with length n. *)
 Axiom bytes : nat -> Type.
 
-Axiom bytes_dec : forall n, EqDec (bytes n).
+Axiom bytes_dec : forall n, EqDec (bytes n) eq.
 
 Existing Instance bytes_dec.
